feat: nonlinear term generation
This is a major refactor of the Bool/Prop simp tester to support other
theories and support non-linear test cases.  As part of this, additional
lemmas were added to improve confluence.

tests/playground/bool_exhaust_test.lean
@@ -1,7 +1,498 @@
-import Lean.Elab.Tactic.ElabTerm
 import Lean.Elab.Command
+import Lean.Elab.Tactic.ElabTerm
+import Lean.Elab.Tactic.Meta
+import Lean.Meta.CheckTactic
+import Lean.Parser.Term
 
 open Lean Lean.Meta Lean.Elab Lean.Elab.Term Lean.Elab.Command
+
+-- | A `Op` is a first order operation for generating values with a given type.
+structure Op (tp : Type) (val : Type) where
+  args : Array tp
+  result : tp
+  apply : Array val → val
+ deriving Inhabited
+
+def mkOp (args : List tp) (result : tp) (apply : Array val → val) : Op tp val :=
+  { apply := apply, args := args.toArray, result }
+
+def Op.map (op : Op x val) (f : x → y) : Op y val :=
+  { apply := op.apply, args := op.args.map f, result := f op.result }
+
+class HasType (val : Type) (type : outParam Type) where
+  typeOf : val → type
+
+class Value (val : Type) where
+  render : val → TermElabM Term
+
+/--
+Contextual information needed to generate terms.
+-/
+structure GenCtx (val : Type) where
+  -- Maps type indices to operator for corresponding type.
+  -- Types use type indices.
+  ops : Array (Array (Op Nat val))
+  /- Operators to use for patterns at top of terms -/
+  topOps : Array (Op Nat val)
+  /-- Maximum term size -/
+  maxTermSize : Nat
+  /-- Maximum depth of terms -/
+  maxDepth : Nat
+  /-- Maximum number of variables -/
+  maxVarCount : Nat
+  /- Local context variables defined in -/
+  lctx : LocalContext
+  /- Local instances for variables -/
+  linst : LocalInstances
+  /-- Maps type indices to variables for that type. -/
+  vars : Array (Array val)
+
+namespace GenCtx
+
+/-- `var ctx tp idx` returns a term denoting `i`th variable with type `tp`. -/
+def var (ctx : GenCtx val) (tp : Nat) (idx : Nat) : Option val :=
+  if g : tp < ctx.vars.size then
+    let a := ctx.vars[tp]'g
+    if h : idx < a.size then
+      some (a[idx]'h)
+    else
+      none
+  else
+    none
+
+end GenCtx
+
+/-- An operator together with a set of terms to apply to it. -/
+structure PartialApp (term : Type) where
+  /-- Operator to generate -/
+  op : Op Nat term
+  /-- Terms constructed so far -/
+  terms : Array term
+
+namespace PartialApp
+
+def fromOp (op : Op Nat term) : PartialApp term :=
+  { op, terms := .mkEmpty op.args.size }
+
+end PartialApp
+
+/--
+A partial term contains the initial part of a term as constructed from a
+left-to-right preorder traversal.
+
+It stores additional information needed to ensure the ultimate term satisfies
+the generation constraints on term size and number of variables.
+
+The operations for constructing this ensures the term is well-formed
+with respect to the signature and is not a complete term.
+-/
+structure PartialTerm (term : Type) where
+  /-- Stack of partially built term (must be non-empty) -/
+  termStack : Array (PartialApp term)
+  /-- Maximum number of additional operations that may be added. -/
+  remTermSize : Nat
+  /-- Variables used with type index. -/
+  usedVars : Array Nat
+  deriving Inhabited
+
+namespace PartialTerm
+
+/--
+Create an initial partial term from an operator.
+
+If the operator is a constant, then this just returns a complete terms.
+-/
+def init (maxTermSize : Nat) (maxDepth : Nat) (op : Op Nat term) : term ⊕ PartialTerm term :=
+  if op.args.isEmpty then
+    .inl (op.apply #[])
+  else
+    .inr {
+      termStack := #[PartialApp.fromOp op],
+      remTermSize := maxTermSize - (1 + op.args.size),
+      usedVars := #[]
+    }
+
+partial def push (p : PartialTerm term) (t : term) : term ⊕ PartialTerm term :=
+  match p.termStack.back? with
+  | none => .inl t
+  | some { op, terms } =>
+    let p := { p with termStack := p.termStack.pop }
+    let terms := terms.push t
+    if terms.size = op.args.size then
+      let v := op.apply terms
+      push p v
+    else
+      .inr { p with termStack := p.termStack.push { op, terms } }
+
+/-- Push an operator to the stack -/
+def pushOp (p : PartialTerm term) (op : Op Nat term) : PartialTerm term :=
+  { termStack   := p.termStack.push (.fromOp op)
+    remTermSize := p.remTermSize - op.args.size,
+    usedVars := p.usedVars
+  }
+
+end PartialTerm
+
+structure State (term : Type) where
+  sofar : Array term := #[]
+  pending : Array (PartialTerm term) := #[]
+  deriving Inhabited
+
+namespace State
+
+def isEmpty (s: State term) : Bool := s.sofar.isEmpty && s.pending.isEmpty
+
+def pop (s : State term) : State term ⊕ (Nat × PartialTerm term × State term) :=
+  if s.pending.isEmpty then
+    .inl s
+  else
+    let { sofar, pending } := s
+    let next := pending.back
+    let pending := pending.pop
+    match next.termStack.back? with
+    | none =>
+      panic! "Term stack empty"
+    | some app =>
+      let tp := app.op.args[app.terms.size]!
+      .inr (tp, next, { sofar, pending })
+
+/- `push s next v` adds the result of `next.push v` to the state. -/
+def push (s : State term) (next : PartialTerm term) (v : term) : State term :=
+  let { sofar, pending } := s
+  match next.push v with
+  | .inl v => { sofar := sofar.push v, pending }
+  | .inr next => { sofar, pending := pending.push next }
+
+def pushOp (s : State term) (ctx : GenCtx term) (next : PartialTerm term) (op : Op Nat term) :=
+  if op.args.isEmpty then
+    s.push next (op.apply #[])
+  else if op.args.size ≤ next.remTermSize ∧ next.termStack.size + 1 < ctx.maxDepth then
+    { s with pending := s.pending.push (next.pushOp op) }
+  else
+    s
+
+def add (s : State term) (val : term ⊕ PartialTerm term) : State term :=
+  let { sofar, pending } := s
+  match val with
+  | .inl v => { sofar := sofar.push v, pending }
+  | .inr p => { sofar, pending := pending.push p }
+
+/-- Create state that will explore all terms in context -/
+def addOpInstances (s : State term) (ctx : GenCtx term) (op : Op Nat term) : State term :=
+  s.add (PartialTerm.init ctx.maxTermSize ctx.maxDepth op)
+
+/-- Create state that will explore all terms in context -/
+def init (ctx : GenCtx term) : State term :=
+  ctx.topOps.foldl (init := {}) (·.addOpInstances ctx ·)
+
+end State
+
+/--
+Generate terms until we reach the limit.
+-/
+partial
+def generateTerms
+    (ctx : GenCtx term)
+    (s : State term)
+    (limit : Nat := 0) :
+    Array term × State term :=
+  if limit > 0 ∧ s.sofar.size ≥ limit then
+    (s.sofar, { s with sofar := #[] })
+  else
+    match s.pop with
+    | .inl s => (s.sofar, { s with sofar := #[] })
+    | .inr (tp, next, s) =>
+      let addVar (next : PartialTerm term) (i : Nat) (s : State term) : State term :=
+            if next.usedVars[i]! = tp then
+              match ctx.var tp i with
+              | some v => s.push next v
+              | none => s
+            else
+              s
+      let s := next.usedVars.size.fold (init := s) (addVar next)
+      let s :=
+        let var := next.usedVars.size
+        if var < ctx.maxVarCount then
+          let next := { next with usedVars := next.usedVars.push tp }
+          addVar next var s
+        else
+          s
+      generateTerms ctx (ctx.ops[tp]!.foldl (init := s) (·.pushOp ctx next ·))
+
+/-
+`addScopeVariables` extends the local context and instances with a copy of the
+variables in the scope (which must be non-empty).
+
+The first variable user name
+
+ extends the local context
+-/
+def addScopeVariables (lctx : LocalContext) (linst : LocalInstances) (scope : Scope) (idx : Nat) :
+    CoreM (LocalContext × LocalInstances × Ident) := do
+  let act := Term.elabBindersEx scope.varDecls fun vars => do pure (vars, ← (read : MetaM Meta.Context))
+  let mctx := { lctx := lctx, localInstances := linst }
+  let (((vars, mctx), _tstate), _mstate) ← act |>.run |>.run mctx
+  if vars.isEmpty then
+    throwError "No variables declared"
+  let fv := vars[0]!.snd |>.fvarId!
+  let rec drop (nm : Name) :=
+        match nm with
+        | .str .anonymous s => pure (.str .anonymous s!"{s}{idx}")
+        | .str nm _ => drop nm
+        | .num nm _ => drop nm
+        | .anonymous => throwError "Anonymous variable declared."
+  let nm ← drop (mctx.lctx.get! fv |>.userName)
+  let lctx := mctx.lctx.setUserName fv nm
+  pure (lctx, mctx.localInstances, mkIdent nm)
+
+def addVariables (cmdCtx : Command.Context) (cmdState : Command.State) (lctx : LocalContext) (linst : LocalInstances) (n : Nat) (cmd : Command) :
+    CoreM (LocalContext × LocalInstances × Array Ident) := do
+  let (_, s) ←  elabCommand cmd.raw |>.run cmdCtx |>.run cmdState
+  let scope := s.scopes.head!
+  Nat.foldM (n := n) (init := (lctx, linst, .mkEmpty n)) fun i (lctx, linst, a) => do
+    let (lctx, linst, ident) ← addScopeVariables lctx linst scope i
+    pure (lctx, linst, a.push ident)
+
+structure VarDecl (tp : Type) where
+  idx : Nat
+  ident : TSyntax `ident
+  type : tp
+  deriving Inhabited, Repr
+
+instance : BEq (VarDecl tp) where
+  beq x y := x.idx == y.idx
+
+instance : Hashable (VarDecl tp) where
+  hash v := hash v.idx
+
+structure GenStats where
+  maxTermSize : Nat := 9
+  maxDepth : Nat := 3
+  maxVarCount : Nat := 3
+
+def mkCtx [BEq tp] [Hashable tp]
+    (types : Array tp)
+    (ops : List (Op tp val))
+    (varGen : List (tp × CoreM Command))
+    (mkVar : VarDecl tp → val)
+    (stats : GenStats)
+    (topOps : List (Op tp val) := ops) : CommandElabM (GenCtx val) := do
+  let typeMap : HashMap tp Nat := Nat.fold (n := types.size) (init := {}) fun i s =>
+        if p : i < types.size then
+          s.insert types[i] i
+        else
+          s
+  let typeFn (t : tp) := typeMap.findD t 0
+  let addOp (a : Array (Array (Op Nat val))) (op : Op tp val) :=
+        let op := op.map typeFn
+        a.modify op.result (·.push op)
+  let init := Array.ofFn (n := types.size) (fun _ => #[])
+  let ops := ops.foldl (init := init) addOp
+  let ops := ops.map (·.reverse)
+  let topOps := topOps.toArray.map (·.map typeFn)
+  let (lctx, linst, vars) ← liftCoreM do
+    let coreCtx ← read
+    let coreState ← get
+    let fileName := coreCtx.fileName
+    let fileMap  := coreCtx.fileMap
+    let env := coreState.env
+    let maxRecDepth := coreCtx.maxRecDepth
+    let cmdCtx : Command.Context := { fileName, fileMap, tacticCache? := none }
+    let cmdState : Command.State := { env, maxRecDepth }
+    let addVars (p : LocalContext × LocalInstances × Array (Array val))
+                (q : tp × CoreM Command) :
+                CoreM (LocalContext × LocalInstances × _) := do
+          let (lctx, linst, a) := p
+          let (type, gen) := q
+          let cmd ← gen
+          let (lctx, linst, vars) ← addVariables cmdCtx cmdState lctx linst stats.maxVarCount cmd
+          let vars := Array.ofFn (n := vars.size) fun j => mkVar { idx := j.val, ident := vars[j], type }
+          let type := typeFn type
+          pure (lctx, linst, a.modify type (fun _ => vars))
+    let vars := Array.ofFn (n := types.size) fun _ => #[]
+    varGen.foldlM (init := ({}, {}, vars)) addVars
+  let maxTermSize : Nat := stats.maxTermSize
+  let maxDepth : Nat := stats.maxDepth
+  let maxVarCount : Nat := stats.maxVarCount
+  pure { ops, topOps, maxTermSize, maxDepth, maxVarCount, lctx, linst, vars }
+
+def State.addOp (s : State val) (ctx : GenCtx val) (op : Op Nat val) : State val :=
+  let {sofar, pending} := s
+  match  PartialTerm.init ctx.maxTermSize ctx.maxDepth op with
+  | .inl v => { sofar := sofar.push v, pending }
+  | .inr gen => { sofar, pending := pending.push gen }
+
+namespace Test
+
+inductive TType where
+| nat
+| int
+deriving BEq, Hashable, Repr
+
+inductive Term where
+| var (v : VarDecl TType)
+| zero
+| succ (x : Term)
+| add (x y : Term)
+deriving Inhabited, Repr
+
+def Term.toString (t:Term) : String :=
+  match t with
+  | .var d => s!"v{d.idx}"
+  | .zero => s!"0"
+  | .succ x => s!"(suc {x.toString})"
+  | add x y => s!"(add {x.toString} {y.toString})"
+
+local syntax:lead (name := myTestElab) "#myTest" : command
+
+@[command_elab myTestElab]
+def elabIntTest : CommandElab := fun _stx => do
+  let types : Array TType := #[.nat, .int]
+  let zeroOp : Op TType Term := Op.mk #[] .nat (fun _ => .zero)
+  let succOp : Op TType Term := Op.mk #[.nat] .nat (fun a => .succ a[0]!)
+  let addOp : Op TType Term := Op.mk #[.nat, .nat] .nat (fun a => .add a[0]! a[1]!)
+  let ops : List (Op TType Term) := [zeroOp, succOp, addOp]
+  let varGen : List (TType × CoreM Command) := [Prod.mk .nat do `(variable (n:Nat))]
+  let stats : GenStats := { maxTermSize := 7, maxDepth := 4, maxVarCount := 3 }
+  let ctx ← mkCtx types ops varGen .var stats
+  let s : State Term := {}
+  let s := s.addOp ctx ctx.ops[0]![1]!
+  let (terms, _) := generateTerms ctx s
+  IO.println s!"Count: {terms.size}"
+  for i in [0:terms.size], t in terms do
+      IO.println s!"  {i}: {t.toString}"
+
+  pure ()
+
+--#myTest
+
+
+end Test
+
+def genOpSubterms (ctx : GenCtx val) (op : Op Nat val) : Array val :=
+  let s : State val := {}
+  let s := s.addOp ctx op
+  let (terms, _) := generateTerms ctx s
+  terms
+
+open Lean.Meta.CheckTactic
+
+def runTests [BEq tp] [HasType val tp] [Value val] (stx : Syntax) (simp : val → val)(tac : Syntax.Tactic) (terms : Array val)
+      : TermElabM Unit := do
+  for tm in terms do
+    if ← IO.checkCanceled then
+      -- should never be visible to users!
+      throw <| Exception.error .missing "Testing interrupted"
+    let res := simp tm
+    let t ← Value.render tm
+    if HasType.typeOf tm != HasType.typeOf res then
+      throwErrorAt stx m!"simp spec for {t} did not preserve type."
+    withoutModifyingEnv $ do
+      let exp ← Value.render res
+      let u ← Lean.Elab.Term.elabTerm t none
+      let type ← inferType u
+      let checkGoalType ← mkCheckGoalType u type
+      let expTerm ← Lean.Elab.Term.elabTerm exp (some type)
+      let mvar ← mkFreshExprMVar (.some checkGoalType)
+      let (goals, _) ← Lean.Elab.runTactic mvar.mvarId! tac.raw
+      match goals with
+      | [next] => do
+        let (val, _, _) ← matchCheckGoalType stx (←next.getType)
+        if !(← Meta.withReducible <| isDefEq val expTerm) then
+          logErrorAt stx
+            m!"{indentExpr u} reduces to{indentExpr val}\nbut is expected to reduce to {indentExpr expTerm}"
+      | [] =>
+        logErrorAt stx
+          m!"{tac} closed goal, but is expected to reduce to {indentExpr expTerm}."
+      | _ => do
+        logErrorAt stx
+          m!"{tac} produced multiple goals, but is expected to reduce to {indentExpr expTerm}."
+
+open Command
+
+private def mkCoreContext (ctx : Command.Context) (options : Options) (maxRecDepth : Nat) (initHeartbeats : Nat) : Core.Context :=
+  { fileName       := ctx.fileName
+    fileMap        := ctx.fileMap
+    options,
+    currRecDepth   := ctx.currRecDepth
+    maxRecDepth,
+    ref            := ctx.ref
+    initHeartbeats,
+    currMacroScope := ctx.currMacroScope }
+
+/-- Runs term elaborator in base context. -/
+def runTermElabM (cctx : Core.Context) (cstate : Core.State) (mctx : Meta.Context) (act : TermElabM Unit)
+    : BaseIO (Except Exception MessageLog) := do
+  let r ← act.run |>.run mctx |>.run cctx cstate |>.toBaseIO
+  match r with
+  | .error e =>
+    pure (.error e)
+  | .ok ((((), _termS), _metaS), coreS) =>
+    pure (.ok coreS.messages)
+
+partial
+def runGen [BEq tp] [Hashable tp] [HasType val tp] [Value val]
+
+      (stx : Syntax) (simp : val → val)
+      (varGen : List (tp × CoreM Command))
+      (mkVar : VarDecl tp → val)
+      (stats : GenStats)
+      (types : Array tp)
+      (ops : List (Op tp val))
+      (tac : Syntax.Tactic)
+      (topOps : List (Op tp val) := ops)
+      (concurrent : Bool := true) : CommandElabM Unit := do
+
+
+  let ctx ← mkCtx (types := types) (ops := ops) (topOps := topOps) (varGen := varGen) (mkVar := mkVar) (stats := stats)
+
+  let lctx := ctx.lctx
+  let linst := ctx.linst
+
+  let cmdCtx : Command.Context ← read
+  let s ← get
+  let ngen := s.ngen
+  let env := s.env
+  let maxRecDepth := s.maxRecDepth
+  let heartbeats ← IO.getNumHeartbeats
+  let options ← getOptions
+  let cctx := mkCoreContext cmdCtx options maxRecDepth heartbeats
+  let cstate : Core.State := { env := env, ngen := ngen, infoState.enabled := false }
+  let mctx : Meta.Context := { lctx := lctx, localInstances := linst }
+  let gen := State.init ctx
+  if concurrent then
+    let limit := 400
+    let rec loop (gen : State val) (tasks : Array (Task (Except Exception MessageLog))) := do
+      if gen.isEmpty then
+        return tasks
+      else
+        IO.println s!"Writing task"
+        let (terms, gen) := generateTerms ctx gen (limit := limit)
+        let t ← runTests stx simp tac terms |> runTermElabM cctx cstate mctx |>.asTask
+        loop gen (tasks.push t)
+    let tasks ←
+      profileitM Exception "simptest.launch" ({} : Options) (decl := .anonymous) do
+        loop gen #[]
+
+    profileitM Exception "simptest.execute" {} do
+      for i in [0:tasks.size] do
+        if ← IO.checkCanceled then
+          break
+        let act := tasks[i]!
+        match act.get with
+        | .error e =>
+          -- Cancel all tasks after this one
+          (tasks |>.toSubarray (start := i+1) |>.forM IO.cancel : BaseIO Unit)
+          throw e
+        | .ok m =>
+          modify fun s => { s with messages := s.messages ++ m }
+  else
+    let r ← runTermElabM cctx cstate mctx <|
+      let (terms, _) := generateTerms ctx gen
+      runTests stx simp tac terms
+    match r with
+    | .error e => throw e
+    | .ok m => modify fun s => { s with messages := s.messages ++ m }
 
 /-
 
@@ -25,7 +516,7 @@ compatiblity.
 inductive BoolType where
   | prop
   | bool
-  deriving BEq, DecidableEq, Inhabited, Repr
+  deriving BEq, DecidableEq, Hashable, Inhabited, Repr
 
 inductive EqOp where
   | eqProp
@@ -89,7 +580,7 @@ particular form of it.
 inductive BoolVal where
   | trueVal (tp : BoolType)
   | falseVal (tp : BoolType)
-  | var (idx : Nat) (v : TSyntax `ident) (tp : BoolType)
+  | var (d : VarDecl BoolType)
     /--
     `(t : Prop)` when `t` is a `Bool`.
 
@@ -113,7 +604,7 @@ def typeOf (v : BoolVal) : BoolType :=
   match v with
   | .trueVal tp => tp
   | .falseVal tp => tp
-  | .var _ _ tp => tp
+  | .var d => d.type
   | .decide _ => .bool
   | .boolToProp _ => .prop
   | .not _ tp => tp
@@ -124,27 +615,13 @@ def typeOf (v : BoolVal) : BoolType :=
   | .ne _ _ op => op.resultType
   | .ite _ _ _ op => op.resultType
 
-structure VarDecl where
-  idx : Nat
-  ident : TSyntax `ident
-  type : BoolType
-
-instance : BEq VarDecl where
-  beq x y := x.idx == y.idx
-
-instance : Hashable VarDecl where
-  hash v := hash v.idx
-
-def render [Monad M] [MonadQuotation M] (v : BoolVal) :
-    StateT (HashSet VarDecl) M (TSyntax `term) :=
+def render [Monad M] [MonadQuotation M] (v : BoolVal) : M Term :=
   match v with
+  | .var d => do pure d.ident
   | .trueVal .bool  => `(true)
   | .trueVal .prop  => `(True)
   | .falseVal .bool => `(false)
   | .falseVal .prop => `(False)
-  | .var idx t tp => do
-    modify (·.insert ⟨idx, t, tp⟩)
-    pure t
   | .boolToProp t => do `(term| ($(←t.render) : Prop))
   | .decide t => do `(term| ($(←t.render) : Bool))
   | .not x .bool => do `(term| !$(←x.render))
@@ -170,7 +647,7 @@ def render [Monad M] [MonadQuotation M] (v : BoolVal) :
 
 def map (f : BoolVal -> BoolVal) (v : BoolVal) : BoolVal :=
   match v with
-  | .trueVal _ | .falseVal _ | .var _ _ _ => v
+  | .trueVal _ | .falseVal _ | .var _ => v
   | .boolToProp t => .boolToProp (f t)
   | .decide t => .decide (f t)
   | .not x tp   => .not (f x) tp
@@ -181,11 +658,6 @@ def map (f : BoolVal -> BoolVal) (v : BoolVal) : BoolVal :=
   | .ne x y op => .ne (f x) (f y) op
   | .ite c x y op => .ite (f c) (f x) (f y) op
 
-def coerceType (v : BoolVal) (type : BoolType) : BoolVal :=
-  match v.typeOf, type with
-  | .prop, .bool => .decide v
-  | .bool, .prop => .boolToProp v
-  | _, _ => v
 
 def trueProp  : BoolVal := .trueVal .prop
 def falseProp : BoolVal := .falseVal .prop
@@ -204,6 +676,32 @@ instance : OrOp BoolVal where
 
 section
 
+@[match_pattern]
+def iff (x y : BoolVal) : BoolVal := .eq x y .iffProp
+
+@[match_pattern]
+def eq_true (x : BoolVal) : BoolVal := .eq x (.trueVal .bool) .eqBool
+
+@[match_pattern]
+def eq_false (x : BoolVal) : BoolVal := .eq x (.falseVal .bool) .eqBool
+
+def toBool (v : BoolVal) : BoolVal :=
+  match v.typeOf with
+  | .prop => .decide v
+  | .bool => v
+
+def toProp (v : BoolVal) : BoolVal :=
+  match v.typeOf with
+  | .prop => v
+  | .bool => eq_true v
+
+def coerceType (v : BoolVal) (type : BoolType) : BoolVal :=
+  match v.typeOf, type with
+  | .prop, .bool => .decide v
+  | .bool, .prop => eq_true v
+  | _, _ => v
+
+
 /--
 Returns true if we should consider `x` a complement of `y`.
 
@@ -215,16 +713,33 @@ def isComplement (x y : BoolVal) : Bool :=
   | x, .not y _ => x == y
   | .eq a b _, .ne c d _ => a.typeOf == c.typeOf && a == b && c == d
   | .ne a b _, .eq c d _ => a.typeOf == c.typeOf && a == b && c == d
+  | eq_true x, eq_false y => x == y
+  | eq_false x, eq_true y => x == y
   | _, _ => false
 
-@[match_pattern]
-def iff (x y : BoolVal) : BoolVal := .eq x y .iffProp
 
-@[match_pattern]
-def eq_true (x : BoolVal) : BoolVal := .eq x (.trueVal .bool) .eqBool
+def resolveEq (thunks : List (term → term → Option term)) (x y : term) : Option term :=
+  match thunks with
+  | [] => none
+  | fn :: thunks =>
+    match fn x y with
+    | none => resolveEq thunks x y
+    | some r => some r
 
-@[match_pattern]
-def eq_false (x : BoolVal) : BoolVal := .eq x (.falseVal .bool) .eqBool
+/--
+Returns true if we should consider `x` a complement of `y`.
+
+Symmetric so also holds if `y` is a complement of `x`.
+-/
+def isOrComplement (x y : BoolVal) (tp : BoolType) : Bool :=
+  match x, y, tp with
+  | .not x _, y, .bool => x == y
+  | x, .not y _, .bool => x == y
+  | .eq a b _, .ne c d _, _ => a.typeOf == c.typeOf && a == b && c == d
+  | .ne a b _, .eq c d _, _ => a.typeOf == c.typeOf && a == b && c == d
+  | eq_true x, eq_false y, _ => x == y
+  | eq_false x, eq_true y, _ => x == y
+  | _, _, _ => false
 
 partial def simp (v : BoolVal) : BoolVal :=
   let v := map simp v
@@ -234,7 +749,7 @@ partial def simp (v : BoolVal) : BoolVal :=
       match p with
       | .trueVal  _ => .trueVal  .bool
       | .falseVal _ => .falseVal .bool
-      | .var _ _ .prop => v
+      | .var _ => v
       | .boolToProp _ => panic! "Expected boolToProp to simplify away"
       | .not x _   => simp <| ~(.decide x)
       | .and x y _ => simp <| (.decide x) &&& (.decide y)
@@ -255,7 +770,7 @@ partial def simp (v : BoolVal) : BoolVal :=
         match op with
         | .iteProp => simp <| .ite c (.decide t) (.decide f) .iteBool
         | _ => v
-      | .var _ _ .bool | .decide _ | .eq _ _ _ =>
+      | .decide _ | .eq _ _ _ =>
         panic! s!"Unexpected prop {repr p} when bool expected."
   | .not t _ =>
     match t with
@@ -299,6 +814,11 @@ partial def simp (v : BoolVal) : BoolVal :=
       else
         return v
   | .or x y tp => Id.run do
+      -- Hardcoded for and-or-imp special case
+      if let .and x1 x2 .prop := x then
+        if let .implies y1 y2 := y then
+          if x1 == y1 then
+            return (simp <| .implies x1 (.or x2 y2 .prop))
       if let .falseVal _ := x then
         return y
       if let .trueVal _ := x then
@@ -313,8 +833,8 @@ partial def simp (v : BoolVal) : BoolVal :=
         if x == yl then return y
       if x == y then
         return x
-      if isComplement x y then
-        return .trueVal tp
+      if isOrComplement x y tp then
+          return .trueVal tp
       pure v
   | .implies x y =>
     match x, y with
@@ -324,10 +844,24 @@ partial def simp (v : BoolVal) : BoolVal :=
     | _, .falseVal _ => simp <| .not x .prop
     | .and a b _, y => simp <| .implies a (.implies b y)
     | x, y => Id.run <| do
-      if let .not y _ := y then
+      if x == y then
+        return (.trueVal .prop)
+      if let eq_true b := x then
+        if let eq_false c := y then
+          if b == c then
+            return y
+      if let eq_false b := x then
+        if let eq_true c := y then
+          if b == c then
+            return y
+      if let .not x _ := x then
         if x == y then
-          return .falseVal .prop
-      return if x == y then .trueVal .prop else v
+          return x
+      if let .not yn _ := y then
+        if x == yn then
+          return y
+
+      return v
   | .eq (.trueVal _) y op =>
     match y with
     | .falseVal _ => .falseVal op.resultType
@@ -350,7 +884,7 @@ partial def simp (v : BoolVal) : BoolVal :=
     (match x with
     | .trueVal _ | .falseVal _ | .implies _ _ | .boolToProp _ =>
       panic! "Unexpected term."
-    | .var _ _ _ => v
+    | .var _ => v
     | .decide t => t
     | .not x _   => simp <| eq_false x
     | .and x y _  => simp <| eq_true x &&& eq_true y
@@ -370,7 +904,7 @@ partial def simp (v : BoolVal) : BoolVal :=
     match x with
     | .trueVal _ | .falseVal _ | .implies _ _ | .boolToProp _ =>
       panic! "Unexpected term."
-    | .var _ _ _ => v
+    | .var _ => v
     | .decide t =>
       simp <| .not t .prop
     | .not x _   =>
@@ -391,6 +925,74 @@ partial def simp (v : BoolVal) : BoolVal :=
       return (.trueVal op.resultType)
     if isComplement x y then
       return (.falseVal op.resultType)
+    if let .beqBool := op then
+      if let .eq x1 x2 .beqBool := x then
+        if x2 == y then
+          return x1
+      if let .eq y1 y2 .beqBool := y then
+        if x == y1 then
+          return y2
+    match op with
+    | .eqProp | .iffProp | .eqBool =>
+      let checks : List (BoolVal → BoolVal → Option BoolVal) := [
+        fun x y =>
+          if let .and x1 x2 _ := x then
+            if x1 == y then
+              some <| .implies (toProp y) (toProp x2)
+            else if x2 == y then
+              some <| .implies (toProp y) (toProp x1)
+            else none
+          else none,
+        fun x y =>
+          if let .and y1 y2 _ := y then
+            if x == y1 then
+              some <| .implies (toProp x) (toProp y2)
+            else if x == y2 then
+              some <| .implies (toProp x) (toProp y1)
+            else none
+          else none,
+        fun x y =>
+          if let .or x1 x2 _ := x then
+            if x1 == y then
+              some <| .implies (toProp x2) (toProp y)
+            else if x2 == y then
+              some <| .implies (toProp x1) (toProp y)
+            else none
+          else none,
+        fun x y =>
+          if let .or y1 y2 _ := y then
+            if x == y1 then
+              some <| .implies (toProp y2) (toProp x)
+            else if x == y2 then
+              some <| .implies (toProp y1) (toProp x)
+            else none
+          else none,
+        fun x y =>
+          if let .or x1 x2 _ := x then
+            if x1 == y then
+              some <| .implies (toProp x2) (toProp y)
+            else if x2 == y then
+              some <| .implies (toProp x1) (toProp y)
+            else none
+          else none,
+        fun x y =>
+          if let .implies x1 x2 := x then
+            if x2 == y then
+              pure <| .or x1 y .prop
+            else none
+          else none,
+        fun x y =>
+          if let .implies y1 y2 := y then
+            if x == y2 then
+              pure <| .or y1 x .prop
+            else none
+          else none
+      ]
+      match resolveEq checks x y with
+      | some r => return (simp r)
+      | none => pure ()
+    | _ =>
+      pure ()
     match op with
     | .eqProp | .iffProp =>
       match x, y with
@@ -423,10 +1025,13 @@ partial def simp (v : BoolVal) : BoolVal :=
       return .falseVal .bool
     if isComplement x y then
       return .trueVal .bool
+    if let .ne y1 y2 .bneBool := y then
+      if x == y1 then
+        return y2
     pure <|
       match x, y with
-      | .ne a b .bneBool, c => .ne a (.ne b c .bneBool) .bneBool
-      | .not x _, .not y _ =>  .ne x y .bneBool
+      | .ne a b .bneBool, c => simp <| .ne a (.ne b c .bneBool) .bneBool
+      | .not x _, .not y _ =>  simp <| .ne x y .bneBool
       | _, _ => v
   | .ite c t f op => Id.run do
     if let .trueVal _ := c then
@@ -435,269 +1040,97 @@ partial def simp (v : BoolVal) : BoolVal :=
       return f
     if let .not c _ := c then
       return simp <| .ite c f t op
-    if let .trueVal tp := t then
-      return simp <| (coerceType c tp) ||| f
     if let .falseVal tp := t then
       return simp <| (~(coerceType c tp)) &&& f
-    if let .trueVal tp := f then
-      return simp <| (~(coerceType c tp)) ||| t
     if let .falseVal tp := f then
       return simp <| (coerceType c tp) &&& t
+    -- NB. The patterns where a branch is true are
+    -- intentionally after branches with a
+    -- false because we prefer to introduce conjunction
+    -- over disjunction/implies when overlapping.
+    if let .trueVal _ := t then
+      let r :=
+        match op with
+        | .iteBool => simp <| toBool c ||| f
+        | .iteProp => simp <| .implies (~c) f
+        | .condBool => simp <|  c ||| f
+        | _ => v
+      return r
+    if let .trueVal _ := f then
+      let r :=
+        match op with
+        | .iteBool  => simp <| ~(toBool c) ||| t
+        | .iteProp  => simp <| .implies c t
+        | .condBool => simp <| ~c ||| t
+        | _ => v
+      return r
     if t == f then
       return t
-    if c == t then
-      return simp <| (coerceType c f.typeOf) ||| f
-    if c == f then
-      return simp <| (coerceType c f.typeOf) &&& t
+    let matchProp c x :=
+          match op with
+          | .iteBool =>
+              if let .decide x := x then
+                if c == x then
+                  some (toBool c)
+                else
+                  none
+              else
+                none
+          | .iteProp | .condBool => if c == x then some c else none
+          | _ => none
+    if let some c := matchProp c t then
+      let r :=
+        match f.typeOf with
+        | .bool => simp <| c ||| f
+        | .prop => simp <| .implies (.not c .prop) f
+      return r
+    if let some c := matchProp c f then
+      return simp <| c &&& t
     let op := match op with
               | .diteProp => .iteProp
               | .diteBool => .iteBool
               | _ => op
     .ite c t f op
-  | .trueVal _ | .falseVal _ | .var _ _ _ => v
+  | .trueVal _ | .falseVal _ | .var _ => v
 end
 set_option profiler false
 
 end BoolVal
 
--- | A `BoolOp` is a datatype capable of generating
-structure BoolOp where
-  args : Array BoolType
-  result : BoolType
-  apply : Array BoolVal → BoolVal
+instance : HasType BoolVal BoolType where
+  typeOf val := val.typeOf
 
-def boolOp
-      (args : Array BoolType)
-      (result : BoolType)
-      (apply : Array BoolVal → BoolVal) : BoolOp :=
-  { apply, args, result }
+instance : Value BoolVal where
+  render val := val.render
 
-def trueOp  (tp : BoolType) : BoolOp := boolOp #[] tp fun _ => .trueVal  tp
-def falseOp (tp : BoolType) : BoolOp := boolOp #[] tp fun _ => .falseVal tp
-def varOp (n : Nat) (v : TSyntax `ident) (tp : BoolType) : BoolOp :=
-  boolOp  #[] .prop fun _ => .var n v tp
-def boolToPropOp : BoolOp := boolOp #[.bool] .prop fun a => .boolToProp (a[0]!)
-def propToBoolOp : BoolOp := boolOp #[.prop] .bool fun a => .decide (a[0]!)
+section
+open BoolVal BoolType
 
-def notOp (tp : BoolType) := boolOp #[tp] tp fun a => .not (a[0]!) tp
-def andOp (tp : BoolType) := boolOp #[tp, tp] tp fun a => .and (a[0]!) (a[1]!) tp
-def orOp  (tp : BoolType) := boolOp #[tp, tp] tp fun a => .or  (a[0]!) (a[1]!) tp
-def impliesOp := boolOp #[.prop, .prop] .prop fun a => .implies  (a[0]!) (a[1]!)
+def trueOp  (tp : BoolType) := mkOp [] tp fun _ => trueVal  tp
+def falseOp (tp : BoolType) := mkOp [] tp fun _ => falseVal tp
+def boolToPropOp := mkOp [.bool] prop fun a => boolToProp (a[0]!)
+def propToBoolOp := mkOp [prop] bool fun a => BoolVal.decide (a[0]!)
+
+def notOp (tp : BoolType) := mkOp [tp] tp fun a => not (a[0]!) tp
+def andOp (tp : BoolType) := mkOp [tp, tp] tp fun a => and (a[0]!) (a[1]!) tp
+def orOp  (tp : BoolType) := mkOp [tp, tp] tp fun a => or  (a[0]!) (a[1]!) tp
+def impliesOp := mkOp [.prop, .prop] prop fun a => implies  (a[0]!) (a[1]!)
 def eqOp  (op : EqOp)  :=
-  boolOp #[op.argType, op.argType] op.resultType fun a => .eq (a[0]!) (a[1]!) op
+  mkOp [op.argType, op.argType] op.resultType fun a => eq (a[0]!) (a[1]!) op
 def neOp  (op : NeOp)  :=
-  boolOp #[op.argType, op.argType] op.resultType fun a => .ne (a[0]!) (a[1]!) op
+  mkOp [op.argType, op.argType] op.resultType fun a => ne (a[0]!) (a[1]!) op
 def iteOp (op : IteOp) :=
   let rtp := op.resultType
-  boolOp #[op.condType, rtp, rtp] rtp fun a => .ite (a[0]!) (a[1]!) (a[2]!) op
+  mkOp [op.condType, rtp, rtp] rtp fun a => ite (a[0]!) (a[1]!) (a[2]!) op
 
-structure GenConfig where
-  maxTermSize : Nat
-  boolOps : List BoolOp
-  propOps : List BoolOp
+end
 
-/--
-State used when generating terms.
+def mkBoolDecl : CoreM Command := `(variable (b : Bool))
+def mkDecidablePropDecl : CoreM Command := `(variable (p : Prop) [Decidable p])
 
-Has control variables needed to know how large the remaining term can be.
+syntax:lead (name := boolTestElab) "#boolTest" : command
 
-Variable identifiers are constructed up front for now.
--/
-structure GenState where
-   -- Size of term including empty slots that need to be populated.
-  termSize : Nat
-  -- Remaining number of variables that can be generated
-  remainingVars : Nat
-  -- Remaining propositional variables available for use in generation.
-  propVars : Array (TSyntax `ident)
-  -- Remaining Boolean variables available for use in generation.
-  boolVars : Array (TSyntax `ident)
-
-@[reducible] def GenM (α : Type) := StateT GenState CommandElabM α
-
-def appendOpApps (cfg : GenConfig) (op : BoolOp)
-     (genTerm : BoolType -> GenState → CommandElabM (Array (BoolVal × GenState)))
-     (r : Array (BoolVal × GenState))
-     (gs : GenState) :
-      CommandElabM (Array (BoolVal × GenState)) := do
-  let newTermSize := gs.termSize + op.args.size
-  if newTermSize > cfg.maxTermSize then
-    pure #[]
-  else
-    -- invariant gs.termSize <= cfg.maxTermSize
-    let gs := { gs with termSize := newTermSize }
-
-    let pushArg (args : Array (Array BoolVal × GenState)) (type : BoolType) := do
-          args.foldlM (init := #[]) fun r (a, gs) => do
-            let terms ← genTerm type gs
-            pure <| terms.foldl (init := r) (fun r (v, gs) => r.push (a.push v, gs))
-
-    let args ← op.args.foldlM (init := #[(#[], gs)]) pushArg
-    pure <| args.foldl (init := r) (fun r (a, gs) => (r.push (op.apply a, gs)))
-
-def genTerm (cfg : GenConfig) (boolOps propOps : List BoolOp) (depth : Nat) (type : BoolType) (gs : GenState) :
-    CommandElabM (Array (BoolVal × GenState)) :=
-  match depth with
-  | 0 =>
-    pure #[]
-  | depth + 1 => do
-    -- Invariant gs.termSize <= cfg.maxTermSize
-    let typedOps :=
-          match type with
-          | .bool => boolOps
-          | .prop => propOps
-    let mkTerm type := genTerm cfg boolOps propOps depth type
-    let r ←
-      if gs.remainingVars > 0 then
-        -- Add vars
-        let n := gs.remainingVars - 1
-        let mut r : Array (BoolVal × GenState) := #[]
-        match type with
-        | .bool =>
-          if gs.boolVars.size > 0 then
-            let v := gs.boolVars.back
-            let gs := { gs with remainingVars := n, boolVars := gs.boolVars.pop }
-            r := r.push (BoolVal.var n v .bool, gs)
-        | .prop =>
-          if gs.propVars.size > 0 then
-            let v := gs.propVars.back
-            let gs := { gs with remainingVars := n, propVars := gs.propVars.pop }
-            r := r.push (BoolVal.var n v .prop, gs)
-        pure r
-      else
-        pure #[]
-
-    typedOps.foldlM (init := r) fun r op =>
-      appendOpApps cfg op mkTerm r gs
-
-section Meta
-
-open Lean
-open Elab.Tactic
-open Meta
-
-/--
-Type used to lift an arbitrary value into a type parameter so it can
-appear in a proof goal.
-
-It is used by the #check_tactic command.
--/
-private inductive CheckGoalType {α : Sort u} : (val : α) → Prop where
-| intro : (val : α) → CheckGoalType val
-
-syntax (name := check_tactic_goal) "check_tactic_goal " term " to " term : tactic
-
-/--
-Implementation of `check_tactic_goal`
--/
-@[tactic check_tactic_goal] private def evalCheckTacticGoal : Tactic := fun stx =>
-  match stx with
-  | `(tactic| check_tactic_goal $src to $exp) => do
-    closeMainGoalUsing (checkUnassigned := true) fun goalType => do
-      let u ← mkFreshLevelMVar
-      let type ← mkFreshExprMVar (.some (.sort u))
-      let src ← Tactic.elabTermEnsuringType src type
-      let val  ← mkFreshExprMVar (.some type)
-      let extType := mkAppN (.const ``CheckGoalType [u]) #[type, val]
-      if !(← isDefEq goalType extType) then
-        throwErrorAt stx "Goal{indentExpr goalType}\nis expected to match {indentExpr extType}"
-      let expTerm ← Tactic.elabTermEnsuringType exp type
-      if !(← Meta.withReducible <| isDefEq val expTerm) then
-        --let src ← Tactic.elabTermEnsuringType src type
-        throwErrorAt stx
-          m!"{indentExpr src} reduces to{indentExpr val}\nbut is expected to reduce to {indentExpr expTerm}\n{toString src}"
-      return mkAppN (.const ``CheckGoalType.intro [u]) #[type, val]
-  | _ => throwErrorAt stx "check_goal syntax error"
-
-end Meta
-
-syntax:lead (name := genTestElab) "#genTest" : command
-
-open Lean.Elab.Command
-
-
-private def addScope : CommandElabM Unit := do
-  let newNamespace ← getCurrNamespace
-  modify fun s => { s with
-    env    := s.env.registerNamespace newNamespace,
-    scopes := { s.scopes.head! with header := "", currNamespace := newNamespace, isNoncomputable := s.scopes.head!.isNoncomputable } :: s.scopes
-  }
-  pushScope
-
-def endScope : CommandElabM Unit := do
-  modify fun s => { s with scopes := s.scopes.drop 1 }
-  popScope
-
-def runTests (stx : Syntax) (cfg : GenConfig) (op : BoolOp) (depth : Nat) (maxVarCount : Nat) : CommandElabM Unit := do
-  let b : TSyntax `ident ← `(b)
-  let c : TSyntax `ident ← `(c)
-  let d : TSyntax `ident ← `(d)
-  let u : TSyntax `ident ← `(u)
-  let v : TSyntax `ident ← `(v)
-  let w : TSyntax `ident ← `(w)
-
-  let genTermC type := genTerm cfg cfg.boolOps cfg.propOps depth type
-  let gs : GenState := {
-          termSize := 1,
-          remainingVars := maxVarCount,
-          boolVars := #[d, c, b],
-          propVars := #[w, v, u]
-        }
-  let terms ← appendOpApps cfg op genTermC #[] gs
-  for (tm, _) in terms do
-    if ← IO.checkCanceled then
-      -- should never be visible to users!
-      throw <| Exception.error .missing "Testing interrupted"
-    let res := tm.simp
-    let (t, decls) ← (tm.render).run {}
-    if tm.typeOf ≠ res.typeOf then
-      logErrorAt stx m!"simp spec for {repr tm} did not preserve type."
-    let (exp, _) ← (res.render).run {}
-    elabCommand (←`(command|section))
-    for ⟨_, nm, tp⟩ in decls do
-      match tp with
-      | .bool =>
-        elabCommand (←`(command|variable ($nm : Bool)))
-      | .prop =>
-        elabCommand (←`(command|variable ($nm : Prop)))
-        elabCommand (←`(command|variable [Decidable $nm]))
-    elabCommand (←`(command|example : CheckGoalType $t := by (try simp); check_tactic_goal $t to $exp))
-    elabCommand (←`(command|end))
-
-def runCommandElabM (ctx : Command.Context) (ngen : NameGenerator) (env : Environment) (maxRecDepth : Nat)
-      (act : CommandElabM Unit) :
-    BaseIO (Except Exception MessageLog) := do
-  let s : Command.State := {
-    env,
-    maxRecDepth,
-    ngen    --nameGenerator
-  }
-  let r ← (act |>.run ctx |>.run s).toBaseIO
-  match r with
-  | .error e =>
-    pure (.error e)
-  | .ok ((), s) =>
-    pure (.ok s.messages)
-
-def runCommandElabM' (acts : List (CommandElabM Unit)) (concurrent := true ) : CommandElabM Unit := do
-  if concurrent then
-    let ctx : Command.Context ← read
-    let s ← get
-    let ngen := s.ngen
-    let env := s.env
-    let maxRecDepth := s.maxRecDepth
-    let acts ← acts.mapM (runCommandElabM ctx ngen env maxRecDepth · |>.asTask)
-    for act in acts do
-      match act.get with
-      | .error e =>
-        throw e
-      | .ok m =>
-        modify fun s => { s with messages := s.messages ++ m }
-    pure ()
-  else
-    acts.forM id
-
-@[command_elab genTestElab]
+@[command_elab boolTestElab]
 def elabGenTest : CommandElab := fun stx => do
   let baseOps := [
       trueOp  .bool,  trueOp .prop,
@@ -715,16 +1148,19 @@ def elabGenTest : CommandElab := fun stx => do
     --iteOp .diteProp,  iteOp .diteBool,
     iteOp .condBool
   ]
+  let types := #[.prop, .bool]
   let ops := baseOps ++ eqOps ++ neOps ++ iteOps
-  let depth := 3
-  let maxVarCount := 3
-  let boolOps := ops.filter (·.result == .bool)
-  let propOps := ops.filter (·.result == .prop)
-  let cfg : GenConfig := { maxTermSize := 9, boolOps, propOps }
+  let varGen : List (BoolType × CoreM Command) := [
+      (.bool, mkBoolDecl),
+      (.prop, mkDecidablePropDecl)
+  ]
+  let stats : GenStats := { maxTermSize := 7, maxDepth := 3, maxVarCount := 2 }
+  let tac : Syntax.Tactic ← `(tactic|try simp)
+  runGen stx BoolVal.simp varGen BoolVal.var stats types ops (topOps := ops) tac
 
-  let runOp op := runTests stx cfg op (depth := depth) (maxVarCount := maxVarCount)
-  -- Note. Can replace ops with a smaller set for specific root
-  -- operators.
-  runCommandElabM' (ops.map runOp)
-
-#genTest
+-- Currently 1.3s
+set_option maxHeartbeats 1000000000
+set_option profiler true
+--set_option profiler.threshold 10
+#boolTest
+set_option profiler false
